Adapt MVCC proof to new string-value interface

etc/update-goose.py
@@ -265,7 +265,7 @@ def main():
             "./tid",
             "./config",
             "./common",
-            "./examples",
+            # "./examples",
             "./tpcc",
             # "./cfmutex",
         )
