src/program_proof/mvcc/wrbuf_prelude.v
@@ -1,13 +1,13 @@
 From Perennial.program_proof.mvcc Require Export mvcc_prelude mvcc_misc mvcc_ghost.
 From Goose.github_com.mit_pdos.go_mvcc Require Export wrbuf.
 
-Definition wrent := (u64 * u64 * bool * loc)%type.
+Definition wrent := (u64 * string * bool * loc)%type.
 
 Definition wrent_to_val (x : wrent) :=
-  (#x.1.1.1, (#x.1.1.2, (#x.1.2, (#x.2, #()))))%V.
+  (#x.1.1.1, (#(LitString x.1.1.2), (#x.1.2, (#x.2, #()))))%V.
 
-Lemma wrent_to_val_unfold (k v : u64) (w : bool) (t : loc) :
-  (#k, (#v, (#w, (#t, #()))))%V = wrent_to_val (k, v, w, t).
+Lemma wrent_to_val_unfold (k : u64) (v : string) (w : bool) (t : loc) :
+  (#k, (#(LitString v), (#w, (#t, #()))))%V = wrent_to_val (k, v, w, t).
 Proof. reflexivity. Qed.
 
 Definition wrent_to_key_dbval (x : wrent) : (u64 * dbval) :=
@@ -17,8 +17,8 @@ Definition wrent_to_key_tpl (x : wrent) : (u64 * loc) :=
   (x.1.1.1, x.2).
 
 Lemma val_to_wrent_with_val_ty (x : val) :
-  val_ty x (uint64T * (uint64T * (boolT * (ptrT * unitT))))%ht ->
-  (∃ (k : u64) (v : u64) (w : bool) (t : loc), x = wrent_to_val (k, v, w, t)).
+  val_ty x (uint64T * (stringT * (boolT * (ptrT * unitT))))%ht ->
+  (∃ (k : u64) (v : string) (w : bool) (t : loc), x = wrent_to_val (k, v, w, t)).
 Proof.
   intros H.
   inversion_clear H. 
@@ -46,7 +46,7 @@ Qed.
 
 Lemma wrent_to_val_with_lookup (x : val) (l : list wrent) (i : nat) :
   (wrent_to_val <$> l) !! i = Some x ->
-  (∃ (k : u64) (v : u64) (w : bool) (t : loc), x = wrent_to_val (k, v, w, t) ∧ l !! i = Some (k, v, w, t)).
+  (∃ (k : u64) (v : string) (w : bool) (t : loc), x = wrent_to_val (k, v, w, t) ∧ l !! i = Some (k, v, w, t)).
 Proof.
   intros H.
   apply list_lookup_fmap_inv in H as [[[[k v] w] t] [Heq Hsome]].
